splitting parital and whole programs in Coq

SemanticsSafetyLike.v
@@ -5,12 +5,13 @@ Require Import CommonST.
 
 Section Main.
 
-Variable prg  : Set.
-Variable ctx  : Set.
-Variable plug : prg -> ctx -> prg.
-
+Variable partial : Set.
+Variable program : Set.
+Variable context : Set.
+Variable plug : partial -> context -> program.
+  
 Variable cfg : Set.
-Variable init : prg -> cfg.
+Variable init : program -> cfg. 
 Variable step : cfg -> event -> cfg -> Prop.
 
 Definition stuck (c:cfg) : Prop :=  forall e c', ~step c e c'.
@@ -19,12 +20,17 @@ CoInductive sem' : cfg -> trace -> Prop :=
 | SStop : forall c, stuck c -> sem' c tstop
 | SCons : forall c e c' t, step c e c' -> sem' c' t -> sem' c (tcons e t).
 
-Definition sem (p:prg) : trace -> Prop := sem' (init p).
+Definition sem (p:program) : trace -> Prop := sem' (init p).
 
 Lemma non_empty_sem : forall P, exists t, sem P t.
 Admitted.
 
-Definition lang : level := @Build_level prg ctx plug sem non_empty_sem.
+Definition lang : level := @Build_level partial
+                                        program
+                                        context
+                                        plug
+                                        sem
+                                        non_empty_sem.
 
 Lemma tgt_sem : semantics_safety_like lang.
 Admitted.
